Tweaking the binary search tree example

teaching/taltech2018/sol/BinarySearchTree.fst
@@ -152,6 +152,11 @@ let rec is_stree (r:mtree) (t:stree) (h:heap) : GTot bool (decreases t) =
                     n = nd.value &&
                     is_stree nd.right t2 h)
 
+let lemma_is_stree_leaf (r:mtree) (h:heap) 
+  : Lemma (requires (is_stree r (empty_stree ()) h))
+          (ensures  (None? (sel h r)))
+  = ()
+
 let rec search (t:erased stree) (r:mtree) (n:nat) 
   : ST bool (requires (fun h0 -> is_stree r (reveal t) h0))
             (ensures  (fun h0 b h1 -> h0 == h1 /\ b = (reveal t) `stree_contains` n)) =
@@ -166,8 +171,8 @@ let rec search (t:erased stree) (r:mtree) (n:nat)
 
 let create () 
   : ST (erased stree * mtree) (requires (fun _ -> True))
-                              (ensures  (fun h0 (t,r) h1 -> //fresh r h0 h1 /\
-                                                            //modifies Set.empty h0 h1 /\
+                              (ensures  (fun h0 (t,r) h1 -> fresh r h0 h1 /\
+                                                            modifies Set.empty h0 h1 /\
                                                             reveal t = empty_stree () /\
                                                             is_stree r (reveal t) h1)) =
   hide Leaf , alloc None
@@ -182,6 +187,15 @@ let rec addrs_of_tree (r:mtree) (t:stree) (h:heap{is_stree r t h})
                              (Set.union (addrs_of_tree nd.left t1 h) 
                                         (addrs_of_tree nd.right t2 h))
 
+let lemma_insert_into_leaf (t:erased stree) (r:mtree) (n:nat) (h0 h1:heap) (r1 r2:mtree)
+  : Lemma (requires (Leaf? (reveal t) /\
+                     is_stree r (reveal t) h0 /\ 
+                     sel h1 r1 == None /\
+                     sel h1 r2 == None /\
+                     sel h1 r == Some ({left = r1; value = n; right = r2})))
+          (ensures  (is_stree r (stree_insert (reveal t) n) h1)) = 
+  ()
+ 
 let rec insert (t:erased stree) (r:mtree) (n:nat) 
   : ST (erased stree) (requires (fun h0 -> is_stree r (reveal t) h0))
                       (ensures  (fun h0 t' h1 -> reveal t' = stree_insert (reveal t) n /\
@@ -189,13 +203,10 @@ let rec insert (t:erased stree) (r:mtree) (n:nat)
                                                  //modifies (addrs_of_tree r (reveal t) h0) h0 h1 /\
   match !r with
   | None -> (
+      recall r;
       let t1,r1 = create () in
       let t2,r2 = create () in  
-      let nd = {left = r1; value = n; right = r2} in
-      assert (Leaf? (reveal t));
-      assert (stree_insert (reveal t) n = Node (reveal t1) n (reveal t2));
-      r := Some nd;
-      admit ();
+      r := Some ({left = r1; value = n; right = r2});
       hide (Node (reveal t1) n (reveal t2)))
   | Some nd -> admit ()
 
